backend/TailcallGotoproof.v
@@ -1,6 +1,7 @@
 Require Import Coqlib Maps Integers AST Linking.
 Require Import Values Memory Events Globalenvs Smallstep.
 Require Import Op Registers RTL Conventions TailcallGoto.
+Require Import TreeProperties Lia.
 
 Definition fenv_compat (p: program) (fenv: funenv) : Prop :=
   forall id f,
@@ -125,104 +126,47 @@ Qed.
 
 Local Open Scope positive_scope.
 
-Definition max_pc_code (co : code) :=
-  PTree.fold (fun m pc i => Pos.max m pc) co 1.
-
-Definition max_pc_list (elts : list (node * instruction)) :=
-  fold_left (fun m pci => Pos.max m (fst pci)) elts 1.
-
-Lemma pos_max_1:
-  forall x, (Pos.max 1 x) = x.
-Proof.
-  intro.
-  apply Pos.max_r.
-  apply Pos.le_1_l.
-Qed.
-
-Lemma max_pc_list_sound1:
-  forall elts: list (node * instruction),
-    elts <> nil ->
-  exists ins : instruction,
-    In ((max_pc_list elts), ins) elts.
-Proof.
-Admitted.
-(*
-  unfold max_pc_list.
-  induction elts; simpl.
-  { congruence. }
-  intros.
-  destruct elts as [ | b rest].
-  { simpl.
-    exists (snd a).
-    unfold max_pc_list.
-    rewrite pos_max_1.
-    left.
-    destruct a; simpl; reflexivity.
-  }
-  generalize 1.
-  assert (b::rest <> nil) as HNIL by congruence.
-  destruct (IHelts HNIL) as [ins1 IN1].
-  
-  intro p.
-  simpl.
-  pose proof (Pos.leb_le (max_pc_list (b::rest)) (fst a)) as HLEB.
-  destruct (Pos.leb (max_pc_list (b::rest)) (fst a)).
-  { exists (snd a).
-    left.
-    unfold max_pc_list in *.
-    simpl.
-    change (max_pc_list (a :: b :: rest)) with
-    (Pos.max (fst a) (max_pc_list (b :: rest))).
-    left.
-   
-  
-  assert (b::rest <> nil) as HNIL by congruence.
-  destruct (IHelts HNIL) as [ins1 IN1].
-  simpl.
-    
-    replace (Pos.max 1 (fst a)) with (fst a) by omega.
- *)
-
-(*
-Lemma max_pc_code_sound1:
-  forall co : code,
-  exists ins : instruction,
-    PTree.get (max_pc_code co) co = Some ins.
-Proof.
-  intros.
-  unfold max_pc_code.
-  rewrite PTree.fold_spec.
-  generalize (PTree.elements co).
- *)
-
-(*
-Definition well_formed_codenode
-  (already : code) (next_node : node) :=
-  next_node = Pos.succ (max_pc_code already).
-
-Lemma generate_moves_wellformed1:
+Lemma generate_moves_respects:
   forall moves : list  (reg * reg),
-  forall pc : node,
   forall jump_point : node,
   forall already : code,
   forall next_node : node,
-    let (already', next_node') := generate_moves pc moves jump_point (already, next_node) in
-    pc < next_node ->
-    well_formed_codenode already next_node ->
-    well_formed_codenode already' next_node'.
+  forall BOUND: strictly_bounds_tree next_node already,
+    let (generated, next_node') := generate_moves moves jump_point already next_node in
+    next_node' > next_node /\
+    forall pc, pc < next_node -> generated!pc = already!pc.
 Proof.
-  induction moves as [ | mh mt Hmt ]; simpl.
+  induction moves; simpl.
+  { intros.
+    split. lia.
+    intros.
+    apply PTree.gso.
+    lia.
+  }
+  destruct a as (src, dst).
+  intros.
+  set (instr := (Iop Omove (src :: nil) dst (Pos.succ next_node))).
+  assert (strictly_bounds_tree (Pos.succ next_node)
+                               (PTree.set next_node instr already)) as BOUND'.
   {
-    intros until next_node.
-    intros BOUNDED WFORMED.
-    unfold well_formed_codenode in *.
-    unfold max_pc_code in *.
-    rewrite PTree.fold_spec in *.
-   }
-    
-  (pc : node) (moves : list (reg * reg))
-           (jump_point : node) (already : code*node) : code*node :=
- *)
+    apply forall_tree_set.
+    lia.
+    apply forall_tree_implies with (P := fun key val => key < next_node).
+    intros; lia.
+    exact BOUND.
+  }
+  pose proof (IHmoves jump_point  (PTree.set next_node instr already)
+                      (Pos.succ next_node) BOUND') as REC.
+  destruct (generate_moves moves jump_point (PTree.set next_node instr already)
+                           (Pos.succ next_node)) as (generated, next_node').
+  destruct REC as (NEXT, PRESERVES).
+  split.
+  lia.
+  intros.
+  rewrite PRESERVES by lia.
+  apply PTree.gso.
+  lia.
+Qed.
 
 (*
 Definition well_formed_tmp (f : function)
